src/MemState/Disk/SimpleDisk.v
@@ -1,3 +1,0 @@
-Require Export GenericDisk.
-
-Definition disk := diskOf block.
